

5.3 Klopferen en vollen  
Klopferen en vollen

$$\mathbb{Z}[i], \mathbb{Z}[\omega]$$

$$\mathbb{Z}[i] = \{a+bi, a, b \in \mathbb{Z}\}$$

$$\mathbb{Q}(i), \mathbb{Q}(\omega)$$

Def:  $F/Q$ ,  $[F:Q] = 2$ ,  $F$  - klopp.

$$F = \mathbb{Q}(\alpha) \quad \alpha - \text{vullen} \quad ax^2 + bx + c \in \mathbb{Z}[x]$$

$$\mathcal{D} = \mathcal{D}_{\mathbb{Q}(\alpha)} - \text{vullen vullen}$$

$$\mathcal{D}_K = \{\alpha \in K : f(\alpha) = 0, f \in \mathbb{Z}[x]\}$$

$$\alpha = \frac{-b \pm \sqrt{b^2 - 4ac}}{2a}$$

$$F = \mathbb{Q}(\sqrt{b^2 - 4ac})$$

$(\mathcal{D} = \mathbb{Z}[\alpha] ? - \text{he vullen vullen})$

$$\mathcal{D} = \mathcal{D}^2 d$$

$$F = \mathbb{Q}(\sqrt{d}), \quad d \in \mathbb{Z}, \quad d \text{ vullen vullen.}$$

$$\text{Gal}(F/Q) \quad ( | \text{Gal}(F/Q) | = [F:Q] )$$

$$\sigma \in G \subset \text{Gal}(F/Q) \quad (\sqrt{d})^2 = d$$

$$(\sigma\sqrt{d})^2 = d \quad \Rightarrow \quad \sigma\sqrt{d} = \pm\sqrt{d}$$

$$\begin{array}{l} \sigma\sqrt{d} = \sqrt{d} \quad \sigma\sqrt{d} = -\sqrt{d} \\ \text{now.} \quad (\text{if } a+ib \mapsto a-ib) \end{array}$$

$$G = \{ \text{id}, \underset{\sigma}{\sqrt{d} \mapsto -\sqrt{d}} \}, \quad F/Q - \text{gen. T. extension}$$

$$\alpha \in F \quad \alpha = r + s\sqrt{d} \quad r, s \in \mathbb{Q}$$

$$\sigma(\alpha) = r - s\sqrt{d} = \alpha' \quad - \text{conj.}$$

$$\text{Tr } \alpha = \alpha + \alpha' = 2r \quad \text{N} \alpha = \alpha \alpha' = r^2 - d s^2$$

$$\text{Lemma: } \alpha \in \mathcal{O} \Leftrightarrow \text{Tr } \alpha, \text{N} \alpha \in \mathbb{Z}$$

$$\square \quad \dots \quad (x - \alpha)(x - \alpha') = x^2 - (\alpha + \alpha')x + \alpha\alpha' \quad \square$$

Proposition:  $\mathcal{D} = \mathcal{D}_{\mathbb{Q}(\sqrt{d})}$

$$\mathcal{D} = \begin{cases} \mathbb{Z}[\sqrt{d}] & d \equiv 1 \pmod{4} \\ \mathbb{Z}\left[\frac{-1+\sqrt{d}}{2}\right] & d \equiv 0 \pmod{4} \end{cases}$$

1)  $\gamma = r + s\sqrt{d} \in \mathcal{D} \iff 2r, r^2 - ds^2 \in \mathbb{Z}$   
 $r, s \in \mathbb{Q} \implies 4ds^2 \in \mathbb{Z} \implies 2s \in \mathbb{Z}$

$m = 2r, n = 2s, m, n \in \mathbb{Z}$

$m^2 - dn^2 = 4(r^2 - ds^2) \equiv 0 \pmod{4}$

$m^2, n^2 \equiv 0, 1 \pmod{4}, d \equiv 1, 2, 3 \pmod{4}$

Case 1

$d \equiv 2 \pmod{4} \quad m^2 - dn^2 \equiv m^2 + 2n^2 \pmod{4}$

$d \equiv 3 \pmod{4} \quad m^2 - dn^2 \equiv m^2 + n^2 \pmod{4}$

$\implies m \equiv n \equiv 0 \pmod{2} \implies r, s \in \mathbb{Z} \implies \mathcal{D} = \mathbb{Z}[\sqrt{d}]$

$$d \equiv 1 \pmod{4} \quad h^2 - d h^2 \equiv h^2 \cdot h^2 \pmod{4}$$

$$\Rightarrow \text{we have } h \equiv 0 \pmod{2} \quad \text{let } h = 2h_1 \pmod{2}$$

$$\Rightarrow \mathcal{D} = \left\{ \frac{1}{2} h + \frac{1}{2} h \sqrt{d} : h \equiv h \pmod{2} \right\}$$

$$\frac{h+h}{2} + h \left( \frac{-1+\sqrt{d}}{2} \right) \Rightarrow \mathcal{D} \subset \underbrace{\mathbb{Z} + \mathbb{Z} \left( \frac{-1+\sqrt{d}}{2} \right)}_{\mathbb{Z} \left[ \frac{-1+\sqrt{d}}{2} \right]}$$

$$\frac{-1+\sqrt{d}}{2} \in \mathcal{D} \Rightarrow \mathbb{Z} \left[ \frac{-1+\sqrt{d}}{2} \right] \subset \mathcal{D}$$

Lemma:  $\delta_F = \text{g.c.d. } F, \delta_F = \begin{cases} 4d, & d \equiv 1, 3 \pmod{4} \\ d, & d \equiv 0, 2 \pmod{4} \end{cases}$

(Note:  $L/K$  is a ...  $L_n \subset L$ )

$$\Delta(\alpha_1, \dots, \alpha_r) = \det \left( \text{Tr}_{L/K}(\alpha_i \alpha_j) \right)$$

$\alpha_i \in \mathcal{O}_K$   $\Delta(\alpha_1, \dots, \alpha_r)$  we can see on below sum)



2)  $e = 1, f = 1, g = 2$  ( $P' = P, P_2, P_1 \neq P$ )  
 $P$  — perpendicular. *perpendicular*

1)  $e = 1, f = 2, g = 1$ , ( $P$ ) =  $\underline{P}$  (чек 2)  
 $P$  — осн. *основание* и  $D$

Теорема:  $P \neq L$  — ч,  $\underline{P}$  — ч и  $D$

$\underline{P}' = \{ \gamma' : \gamma \in \underline{P} \} = \{ r - s\sqrt{d} : r + s\sqrt{d} \in \underline{P} \}$

1)  $\left( \frac{\delta_F}{P} \right) = 0$  (ч.  $P \mid \delta_F$ ) : ( $P$ ) =  $\underline{P}^2$

2)  $\left( \frac{\delta_F}{P} \right) = 1$  ( $P \nmid \delta_F$ ) ( $P$ ) =  $\underline{P} \cdot \underline{P}'$ ,  $P \neq P'$

3)  $\left( \frac{\delta_F}{P} \right) = -1$  ( $P \nmid \delta_F$ ) ( $P$ ) =  $\underline{P}$

$\square$  1)  $P \mid \delta_F$   $\delta_F = \begin{cases} 4d \\ d \end{cases} \Rightarrow P \mid d$ .

Итак  $\underline{P} = (P, \sqrt{d}) = \{ 2P + \mu\sqrt{d} \}$  — ч. и  $D$

$$P^2 = (p, \sqrt{d})(p, \sqrt{d})$$

$$(a, p+1, \sqrt{d}, (2p+1, \sqrt{d})) =$$

$$= p^2 a_1 a_2 + (a_1 p_1 + p_1 a_2) p \sqrt{d} + p_1 p_2 d =$$

$$= p (p a_1 a_2 + (a_1 p_1 + p_1 a_2) \sqrt{d} + p_1 p_2 \frac{d}{p}) \in$$

$$(p) \left( p, \sqrt{d}, \frac{d}{p} \right)$$

$$\underbrace{\quad}_{= \bar{1}} \leftarrow \gamma_1 p + \gamma_2 \sqrt{d} + \gamma_3 \frac{d}{p}, \gamma_i \in \mathcal{D}$$

$$(p, \frac{d}{p}) \in I \Rightarrow \gamma p + \gamma_3 \frac{d}{p} = 1 \in I$$

$$\Rightarrow \bar{1} \in \mathcal{D}$$

$$(p, \sqrt{d})^2 = P^2 \subset (p) \Rightarrow (p) \mid P^2$$

$$P = (p, \sqrt{d}) \Rightarrow (p) \neq P$$

$$P \neq \text{m.h.} \quad (\text{no e.f.s.}) \quad (p) \neq P^2$$

2)  $\left(\frac{S_{1-}}{p}\right) \geq 1$   $\Leftrightarrow$  2)  $\left(\frac{d}{p}\right) \geq 1$   $\Leftrightarrow$  2)  $\exists a \in \mathbb{Z} : a^2 \equiv d \pmod{p}$

$$P = (p, a + \sqrt{d}) \quad , \quad P' = (p, a - \sqrt{d})$$

$$P, P' \subset (P) \left( \underbrace{p, a + \sqrt{d}, a \cdot \sqrt{d}}_{\in I}, \frac{a^2 - d}{p} \right)$$

$$2a \quad \text{"} \quad a + \sqrt{a} + a - \sqrt{a} \in \mathbb{I} \quad , \quad p \in \mathbb{I}$$

4.  $(p, 2a, 2, 2) \dots 2, 1 \in \mathbb{Z} \Rightarrow \mathbb{Z}^2 \cong \mathbb{D}$

$$\mathcal{P}, \mathcal{P}' \subset (\mathcal{P})$$

$$\Sigma \ll \underline{P} \geq \underline{P}' \quad (p, a + \sqrt{d}, z) (p, a - \sqrt{d})$$

2) P. Lac P 2) P 2D - X

$$2, \quad P \neq P'$$



$$\underline{P} \cdot P' \subset (P) \quad \Leftrightarrow, \quad (P') \mid P P'$$

$$(P') \not\subset \underline{P} \quad \neq \underline{P}' \quad \Leftrightarrow, \quad (P') \neq P \cdot P'$$

$$1) \left( \frac{\delta^2}{P} \right) = -1 \quad \Leftrightarrow, \quad \left( \frac{d}{P} \right) = -1$$

$$\underline{P} \mid (P), \quad (P') \subset \underline{P}$$

$$|D/P| = p^f, \quad f = 1, 2$$

$$\text{In } |D/P| = p$$

$$\frac{\mathbb{Z}}{p} \mid p \mathbb{Z} \hookrightarrow \frac{D}{P} \quad \Leftrightarrow, \quad \forall \bar{2} \in D/P \quad \exists a \in \mathbb{Z}:$$

$$\bar{2} \equiv a (P)$$

$$2 \equiv \sqrt{d} \quad \exists a, \quad a \equiv \sqrt{d} (P)$$

$$\Leftrightarrow, \quad a^2 \equiv d (P)$$

$$a^2 - d \in \mathbb{P}$$

$$\in \mathbb{A}$$

$$\mathbb{P} \cap \mathbb{A} = \{1\}$$

$$2) \quad a^2 - d \in (\mathbb{P})$$

$$a^2 \equiv d \pmod{\mathbb{P}}$$

$$- > < \left(\frac{d}{p}\right) = -1$$

$$2) \quad f = 2$$

$$(\mathbb{P}) = \mathbb{P}$$

$$1 \in \mathbb{D} \quad \square$$

Hege:  $f = 2$

$$1) \quad 2 \mid \delta_i \quad 2) \quad (2) = \mathbb{P}^2$$

$$2) \quad 2 \nmid \delta_i \quad d \equiv 1 \pmod{2} \quad 2) \quad (2) = \mathbb{P} \mathbb{P}' \quad \mathbb{P} \neq \mathbb{P}'$$

$$3) \quad 2 \nmid \delta_i \quad d \equiv 5 \pmod{8} \quad 2) \quad (2) = \mathbb{P}$$

$\square$  ..  $\square$

$$\mathbb{P} \text{ von } \mathbb{P} \quad \mathbb{P} \in \mathbb{D}^* \quad (23) \quad (2)$$

$$\mathbb{P} \neq \mathbb{P}'$$

Theorem:  $d < 0$ ,  $U_d = D^*$  - yes es.

1)  $U_{-1} = \{ \pm 1, \pm i \}$  :  $|U_{-1}| = 4$

2)  $U_{-1} = \{ \pm 1; \pm \omega; \pm \omega^2 \}$   $\omega = \frac{-1 + \sqrt{-3}}{2}$   
 $|U_{-1}| = 6$

3)  $U_d = \{ \pm 1 \}$ ,  $d < -1$ ,  $d = -2$

$\square$   $d \in \{2, 3, 4\}$   $D = \mathbb{Z}[\sqrt{d}]$

$x \neq y \sqrt{d} \in D$  - es  $(\Rightarrow) x^2 - dy^2 = \pm 1$

$x^2 + |d|y^2 = 1$

es  $|d| > 1$ , no sol  $(x, y) = (\pm 1, 0)$

es  $|d| = 1$ ,  $d = -1$ ,  $\mathbb{Z}[i]$ , sol  
 $(\pm 1, 0), (0, \pm 1)$

$$d \in (4) \quad , \quad \mathcal{D}: 2x + 5 = \frac{-1 \pm \sqrt{d}}{2}$$

$$2x - 5 + 5\sqrt{d} = \frac{2 \pm 5\sqrt{d}}{2}$$

$$2 \mid 5 \quad (2)$$

$$d = 1 \quad (2) \quad 2^2 - d \cdot 5^2 = 4 \quad , \quad d < 0$$

$$(2) \quad 2^2 + |d| \cdot 5^2 = 4 \quad , \quad |d| > 3$$

$$|d| > 2 \quad d = -3 \quad x^2 + 3y^2 = 4 \quad - (*)$$

Theorem (See 5.16)  $d > 0$   $\mathcal{D}$

Seh.  $u \in \mathcal{D}$  - gr. g.

$$d \quad : \quad N_d = \{ \pm \varepsilon^m \cdot u \in \mathcal{D} \}$$

(gsm  $x^2 - dy^2 = 1$  - Pell's equation)

Theorem (Dirichlet 2.18):  $\exists$  — unique  
rational  $\gamma$  such that  $\sum \gamma : Q) = 4$ .

Chap. 7. 2. 2.

$$U_D = \sum_{\alpha} \left( \frac{1}{2} \epsilon_{\alpha}^{\dagger} \epsilon_{\alpha} + \frac{1}{2} \epsilon_{\alpha} \epsilon_{\alpha}^{\dagger} \right) - g \psi$$

17 D-6, A-II 12

## Kosten der Warte

$$h \in \mathbb{Z}_{>0} \quad S = S_h = e^{2\pi i \frac{1}{h}}, \quad X^{h-1}$$

Q4.  $F = \mathcal{O}(S_m)$   $n \leq$   $n - 62$   $n$   $n$

$$x^n - 1 = (x - s)(x - s^2) \cdots (x - s^{n-1})(x - s^{\frac{n}{2}})$$

$$= \prod_{i=1}^n (x - s^i)$$

$\mathbb{Q}(s)$  - ~~real~~ <sup>complex</sup> ~~number~~ <sup>field</sup>.

$\mathbb{Q}(s)/\mathbb{Q}$  - ~~extension~~ <sup>extension</sup> ~~field~~ <sup>field</sup>.

Def.  $\phi_n(x) = \prod_{(a,n)=1} (x - s^a)$ ,  $\deg \phi_n = \phi(n)$

Lemma :  $x^n - 1 = \prod_{d|n} \phi_d(x)$

Proof ~~Since~~ <sup>Since</sup> ~~we have~~ <sup>we have</sup>  $1 = \prod_{d|n} \phi_d(x)$  (2)

Lemma :  $\phi_n \in \mathbb{Z}[x]$

Proof ~~Since~~ <sup>Since</sup> ~~we have~~ <sup>we have</sup>  $\phi_n(x) = \prod_{(a,n)=1} (x - s^a)$

$$\text{Gal}(\mathbb{Q}(\zeta)/\mathbb{Q}) \cong G_m$$

Lemma:  $\exists \theta: G_m \rightarrow \text{Aut}(\mathbb{Z}/n\mathbb{Z})$  - unique  
 versch.  $\gamma \in G_m$

$$\square \quad \zeta^n = 1, \quad \sigma \in G_m, \quad (\sigma \zeta)^n = 1 \quad \Rightarrow$$

$$\left( \zeta = e^{2\pi i \frac{1}{n}}, \quad \zeta_a = e^{2\pi i \frac{a}{n}} \right) \quad \sigma \zeta = \zeta^a$$

$$\theta \in \mathbb{Z}/n\mathbb{Z} \quad \theta = \theta(\sigma)$$

$$\tau = \sigma^{-1} \quad \tau \sigma = \text{id} \quad (\tau \sigma)(\zeta) = \zeta$$

$$\tau(\sigma(\zeta)) = \tau(\zeta^{\theta(\sigma)}) = \zeta^{\theta(\tau, \theta(\sigma))}$$

$$= (\tau \zeta)^{\theta(\sigma)} = \zeta^{\theta(\tau, \theta(\sigma))}$$

$$\Rightarrow \theta(\zeta, \theta(\sigma)) = \tau(m)$$

$$\sigma_1, \sigma_2 \in G_m \quad \sigma_1(\sigma_2(\zeta)) = (\sigma_1 \sigma_2)(\zeta) = \zeta^{\theta(\sigma_1, \sigma_2)}$$

$$\stackrel{\theta(\sigma_1, \theta(\sigma_2))}{=} \zeta^{\theta(\sigma_1, \theta(\sigma_2))} \quad \Rightarrow \quad \theta(\sigma_1 \sigma_2) = \theta(\sigma_1) \theta(\sigma_2)$$

$$(4)$$

Unerwünscht:  $\theta(\sigma) = 1 \quad (\sigma = \text{id}) \quad \sigma \zeta = \zeta^{\theta(\sigma)} = \zeta$

$$\sigma = \text{id}$$

$$\theta \quad \text{ist} \quad \text{in} \quad \text{Aut}(\mathbb{Z}/n\mathbb{Z}) \quad \square$$

$\mathbb{Q}(s)/\mathbb{Q}$  - Lehmer. ,

Lehmer Trough

Proposition :  $\mathbb{Q}(s)/\mathbb{Q}$  - Lehmer Trough

$$\sum \mathbb{Q}(s) : \mathbb{Q} \approx |G_n|$$

Lemma :  $|G_n| \mid \varphi(n) \quad \square \mid \mathbb{Z} \mid \mathbb{Z} \mid \approx \varphi(n) \mid \mathbb{Z}$

Lemma :  $\varphi_n \in \mathbb{Z}[X]$

1)  $\sigma \varphi_n(X) \approx \sigma(\prod_{(a,n)=1} (X - s^a)) \approx$

$\approx \prod_{(a,n)=1} (X - s^{a \cdot B(s)}) \approx \varphi_n(X)$

$\Rightarrow \varphi_n \in \mathbb{Q}[X], \in \mathbb{Z}[X] \quad \square$



Theorem:  $\phi_n(x)$  is irr. /  $\mathbb{Q}$  (1.1)

$\square$  <sup>user:</sup>  $\phi_n$  - irr. show  $\exists$  s.t.  $\mathbb{Q}(\zeta)$

irr.  $\mathbb{Q}$  - irr. show  $\exists$ ,  $p = 1$ .

(p. 1) = 1

$$\mathbb{D} = \mathbb{D}_{\mathbb{Q}(\zeta)}$$

$(p) \subset \mathbb{I}^p$  - irr. w.r.t.  $\mathbb{D}$   
 , has  $p$

$\mathbb{Q}$  irr.  $\exists$  - irr.  $X^n - 1 \Rightarrow \mathbb{Q} \mid X^n - 1$

$\mathbb{Z}$ , irr.  $\mathbb{Q}$  irr.  $\mathbb{Q}$  irr.  $X^n - 1$   
 m.c.  $\sqrt[n]{1}$  (same as  $X^n - 1$ )

$$\Delta = \prod_{i < j} (s^i - s^j)^2 = \pm \prod_{i \neq j} (s^i - s^j) = \pm \prod_{i \neq 0} s^i (1 - s^{j-i})$$

$$= \pm \prod_i s^i \prod_{k \neq 0} (1 - s^k)$$

$$\frac{x^m - 1}{x - 1} = \prod_{k \neq 0} (x - s^k)$$

$$x^{m-1} + x^{m-2} + \dots + 1$$

$$\text{Für } m = 1 \quad 1 \quad m = \prod_{k \neq 0} (1 - s^k)$$

$$D = \pm \prod_i (s^{i, m}) = \pm m^m \prod_{i=1}^m s^i = \pm m^m$$

$$|D| = m^m$$

$$(p, m) = 1 \quad s^r - \text{non zero } f :$$

$$\text{wenn } f(s^r) \neq 0$$

$$f(x) = (x - s_1) \dots (x - s_k) \quad s_i = s = e^{2\pi i \frac{1}{m}}$$

$$f(s^p) = \prod (\text{element in } (s^i - s^j))$$

$$2) \quad f(s^p) \mid \Delta \quad \text{and} \quad \mathcal{D}$$

$$2) \quad f(s^p) \mid m^n \quad \text{and} \quad \mathcal{D}$$

$$f(x^p) \equiv f(x)^p \pmod{p} \quad p \mid f(x^p) - f(x)^p$$

$$f(s^p) \equiv f(s)^p \pmod{p} \quad \text{and} \quad \mathcal{D}$$

$$\text{and} \quad \mathcal{D} \quad p \mid f(s^p) \mid m^n$$

$$2) \quad p \mid m^n \quad \text{and} \quad \mathcal{D} \quad \Rightarrow \quad p \mid m^2 \quad \text{and} \quad \mathcal{D}$$

$$- \quad > < \quad (p, m) \geq 1$$

$$\text{Ex. 2.} \quad f(s^p) = 0$$

$$S \in (a, \infty) \subset \mathbb{R} \quad a = \prod p_i^{v_i} \quad (p_i \nmid a, v_i = 1)$$

$$\Rightarrow S^a = \text{norm} \text{ von } L$$

$$\deg L \geq \varphi(a)$$

$$\phi_n(S) = 0 \quad \Rightarrow \quad L \mid \phi_n \quad \Rightarrow \quad \deg L \leq \varphi(n)$$

$$\deg L = \deg \phi_n = \varphi(n)$$

$$L \subset \phi_n \subset \prod_{(a, n, 2)} (x + S^a)$$

$$\Rightarrow \phi_n \text{ irreduzibel.} \quad (2)$$

$$\underline{\text{Lemma 1}} \quad (1) \quad \{Q(S, i, Q)\} = \varphi(n)$$

$$(2) \quad \psi: \mathbb{Q}_n \rightarrow K(\mathbb{F}_n, \mathbb{F}) \quad - \quad \text{isom}$$

Теорема :  $D \cong \mathbb{Z}[S]$

(  $p$  - чет.,  $m = p - 2$ . )

$Q(2)$ ,  $D_{Q(2)} \neq \mathbb{Z}[S]$

Лемма :  $p \times n$ ,  $I$  - чет.  $p$  mod 2  
(  $p^2 \leq 1(m)$ ,  $I$  - чет. )  $\Rightarrow D$

(  $p$  )  $= I_1, \dots, I_g$ ,  $I_i$  - чет.,  $I$

$$D = \frac{\varphi(n)}{I}$$

$\square$   $\dots$   $\square$

Лемма :  $p \times n$   $I^p \cong (1-S)$  ( $S \cong S_p \cong e^{2\pi i \frac{1}{p}}$ )  
 $p$  - чет.  $\Rightarrow D$  ( $p$ )  $= I^{p-1}$   $\square$   $\dots$   $\square$

$$\{ \mathbb{R} \}$$

$$d < 0$$

$$i, \omega, \frac{-1 + \sqrt{3}}{2}$$

2

work in ...

Therefore (by the ... )  $\forall F/Q$  -  
 $\text{rank}(F/Q) = \text{rank}(S_n)$

where

$\Rightarrow$

$$F \subset Q(S_n)$$

$$S_n \neq \mathbb{C}$$

$$S_n \neq \frac{1}{2}$$

$$Q(S_n)/F/Q$$

C

D

$\mathbb{R}^n$

$$\{ \mathbb{R} \}$$

